src/n-bit/bitScript.sml
@@ -6,13 +6,27 @@
 (* ========================================================================= *)
 
 (* interactive use:
-  load "logrootTheory";
+  app load ["logrootTheory","stringLib"];
 *)
 
-open HolKernel Parse boolLib bossLib;
-open Q simpLib numLib arithmeticTheory logrootTheory prim_recTheory;
+open HolKernel Parse boolLib bossLib Q simpLib numLib stringLib;
+open arithmeticTheory listTheory rich_listTheory stringTheory
+     logrootTheory prim_recTheory;
 
 val _ = new_theory "bit";
+
+(* ------------------------------------------------------------------------- *)
+
+infix \\ << >>
+
+val op \\ = op THEN;
+val op << = op THENL;
+val op >> = op THEN1;
+
+val LEFT_REWRITE_TAC =
+  GEN_REWRITE_TAC (RATOR_CONV o DEPTH_CONV) empty_rewrites;
+
+val POP_LAST_TAC = POP_ASSUM (K ALL_TAC);
 
 (* ------------------------------------------------------------------------- *)
 
@@ -62,23 +76,89 @@ val MOD_2EXP_EQ_def = Define`
 val MOD_2EXP_MAX_def = Define`
   MOD_2EXP_MAX n a = (MOD_2EXP n a = (2 ** n - 1))`;
 
+val _ = computeLib.auto_import_definitions := true;
+
+val l2n_def = Define`
+  (l2n b [] = 0) /\
+  (l2n b (h::t) = h MOD b + b * l2n b t)`;
+
+val n2l_def = Define`
+  n2l b n = if n < b \/ b < 2 then [n MOD b] else n MOD b :: n2l b (n DIV b)`;
+
+val s2n_def = Define `s2n b f s = l2n b (MAP f (REVERSE (EXPLODE s)))`;
+val n2s_def = Define `n2s b f n = IMPLODE (REVERSE (MAP f (n2l b n)))`;
+
+val HEX_def = Define`
+  (HEX 0 = #"0") /\
+  (HEX 1 = #"1") /\
+  (HEX 2 = #"2") /\
+  (HEX 3 = #"3") /\
+  (HEX 4 = #"4") /\
+  (HEX 5 = #"5") /\
+  (HEX 6 = #"6") /\
+  (HEX 7 = #"7") /\
+  (HEX 8 = #"8") /\
+  (HEX 9 = #"9") /\
+  (HEX 10 = #"A") /\
+  (HEX 11 = #"B") /\
+  (HEX 12 = #"C") /\
+  (HEX 13 = #"D") /\
+  (HEX 14 = #"E") /\
+  (HEX 15 = #"F")`;
+
+val UNHEX_def = Define`
+  (UNHEX #"0" = 0) /\
+  (UNHEX #"1" = 1) /\
+  (UNHEX #"2" = 2) /\
+  (UNHEX #"3" = 3) /\
+  (UNHEX #"4" = 4) /\
+  (UNHEX #"5" = 5) /\
+  (UNHEX #"6" = 6) /\
+  (UNHEX #"7" = 7) /\
+  (UNHEX #"8" = 8) /\
+  (UNHEX #"9" = 9) /\
+  (UNHEX #"a" = 10) /\
+  (UNHEX #"b" = 11) /\
+  (UNHEX #"c" = 12) /\
+  (UNHEX #"d" = 13) /\
+  (UNHEX #"e" = 14) /\
+  (UNHEX #"f" = 15) /\
+  (UNHEX #"A" = 10) /\
+  (UNHEX #"B" = 11) /\
+  (UNHEX #"C" = 12) /\
+  (UNHEX #"D" = 13) /\
+  (UNHEX #"E" = 14) /\
+  (UNHEX #"F" = 15)`;
+
+val num_from_bin_list_def = Define `num_from_bin_list = l2n 2`;
+val num_from_oct_list_def = Define `num_from_oct_list = l2n 8`;
+val num_from_dec_list_def = Define `num_from_dec_list = l2n 10`;
+val num_from_hex_list_def = Define `num_from_hex_list = l2n 16`;
+
+val num_to_bin_list_def = Define `num_to_bin_list = n2l 2`;
+val num_to_oct_list_def = Define `num_to_oct_list = n2l 8`;
+val num_to_dec_list_def = Define `num_to_dec_list = n2l 10`;
+val num_to_hex_list_def = Define `num_to_hex_list = n2l 16`;
+
+val num_from_bin_string_def = Define `num_from_bin_string = s2n 2 UNHEX`;
+val num_from_oct_string_def = Define `num_from_oct_string = s2n 8 UNHEX`;
+val num_from_dec_string_def = Define `num_from_dec_string = s2n 10 UNHEX`;
+val num_from_hex_string_def = Define `num_from_hex_string = s2n 16 UNHEX`;
+
+val num_to_bin_string_def = Define `num_to_bin_string = n2s 2 HEX`;
+val num_to_oct_string_def = Define `num_to_oct_string = n2s 8 HEX`;
+val num_to_dec_string_def = Define `num_to_dec_string = n2s 10 HEX`;
+val num_to_hex_string_def = Define `num_to_hex_string = n2s 16 HEX`;
+
+(* ------------------------------------------------------------------------- *)
+
+val LOG_RWT = store_thm("LOG_RWT",
+  `!m n. 1 < m /\ 0 < n ==>
+     (LOG m n = if n < m then 0 else SUC (LOG m (n DIV m)))`,
+  SRW_TAC [ARITH_ss] [LOG_DIV, ADD1, LOG_UNIQUE, EXP]);
+
 val LOG2_UNIQUE = save_thm("LOG2_UNIQUE",
   (REWRITE_RULE [GSYM LOG2_def] o INST [`a` |-> `2`]) LOG_UNIQUE);
-
-(* ------------------------------------------------------------------------- *)
-
-infix \\ << >>
-
-val op \\ = op THEN;
-val op << = op THENL;
-val op >> = op THEN1;
-
-val LEFT_REWRITE_TAC =
-  GEN_REWRITE_TAC (RATOR_CONV o DEPTH_CONV) empty_rewrites;
-
-val POP_LAST_TAC = POP_ASSUM (K ALL_TAC);
-
-(* ------------------------------------------------------------------------- *)
 
 val DIVMOD_2EXP = save_thm("DIVMOD_2EXP",
   REWRITE_RULE [GSYM DIV_2EXP_def,GSYM MOD_2EXP_def] DIVMOD_2EXP_def);
@@ -1032,6 +1112,270 @@ val BIT_SIGN_EXTEND = store_thm("BIT_SIGN_EXTEND",
       Cases_on `l`
         \\ FULL_SIMP_TAC arith_ss
              [MIN_DEF, GSYM BITS_ZERO3, BITS_ZERO, BIT_def, BITS_COMP_THM2]]);
+
+(* ------------------------------------------------------------------------- *)
+
+val LENGTH_n2l = store_thm("LENGTH_n2l",
+  `!b n. 1 < b ==> (LENGTH (n2l b n) = if n = 0 then 1 else SUC (LOG b n))`,
+  completeInduct_on `LOG b n`
+    \\ SRW_TAC [ARITH_ss] [Once n2l_def, LOG_RWT]
+    \\ SRW_TAC [ARITH_ss] [LOG_RWT]
+    \\ `0 < n DIV b` by SRW_TAC [ARITH_ss] [X_LT_DIV]
+    \\ DECIDE_TAC);
+
+val LOG_DIV_LESS = prove(
+  `!b n. b <= n /\ 1 < b ==> LOG b (n DIV b) < LOG b n`,
+  SRW_TAC [] [] \\ IMP_RES_TAC LOG_DIV \\ DECIDE_TAC);
+
+val l2n_n2l = store_thm("l2n_n2l",
+  `!b n. 1 < b ==> (l2n b (n2l b n) = n)`,
+  completeInduct_on `LOG b n`
+    \\ SRW_TAC [ARITH_ss] [Once n2l_def, l2n_def]
+    \\ `LOG b (n DIV b) < LOG b n` by SRW_TAC [ARITH_ss] [LOG_DIV_LESS]
+    \\ SRW_TAC [ARITH_ss] [(GSYM o ONCE_REWRITE_RULE [MULT_COMM]) DIVISION]);
+
+(* ......................................................................... *)
+
+val LENGTH_l2n = store_thm("LENGTH_l2n",
+  `!b l. 1 < b /\ EVERY ($> b) l /\ ~(l2n b l = 0) ==>
+     (SUC (LOG b (l2n b l)) <= LENGTH l)`,
+  Induct_on `l` \\ SRW_TAC [ARITH_ss] [l2n_def, GREATER_DEF]
+    << [ALL_TAC, `~(h = 0)` by (`0 < b` by DECIDE_TAC \\ STRIP_TAC
+          \\ IMP_RES_TAC ZERO_MOD \\ FULL_SIMP_TAC arith_ss [])]
+    \\ `0 < h + b * l2n b l`
+    by (IMP_RES_TAC (simpLib.SIMP_PROVE arith_ss [LESS_MULT2]
+         ``1 < b /\ ~(c = 0) ==> 0 < b * c``) \\ SRW_TAC [ARITH_ss] [])
+    \\ SRW_TAC [ARITH_ss] [LOG_RWT, LESS_DIV_EQ_ZERO,
+         SIMP_RULE arith_ss [] ADD_DIV_ADD_DIV]
+    << [Cases_on `l` \\ FULL_SIMP_TAC (arith_ss++listSimps.LIST_ss) [l2n_def],
+        SRW_TAC [ARITH_ss] [(GSYM o REWRITE_RULE [GSYM SUC_ONE_ADD]) LOG_DIV],
+        `~(l2n b l = 0)` by (STRIP_TAC \\ FULL_SIMP_TAC arith_ss [])
+          \\ SRW_TAC [] []]);
+
+val EL_TAKE = store_thm("EL_TAKE",
+  `!x n l. x < n /\ n <= LENGTH l ==> (EL x (TAKE n l) = EL x l)`,
+  Induct_on `l` \\ Cases_on `x` \\ SRW_TAC [ARITH_ss] []);
+
+val l2n_DIGIT = store_thm("l2n_DIGIT",
+  `!b l x. 1 < b /\ EVERY ($> b) l /\ x < LENGTH l ==>
+      ((l2n b l DIV b ** x) MOD b = EL x l)`,
+  Induct_on `l` \\ SRW_TAC [ARITH_ss] [l2n_def, GREATER_DEF]
+    \\ Cases_on `x`
+    \\ SRW_TAC [ARITH_ss]
+        [EXP, GSYM DIV_DIV_DIV_MULT, ZERO_LT_EXP, LESS_DIV_EQ_ZERO,
+         SIMP_RULE arith_ss [] (CONJ MOD_TIMES ADD_DIV_ADD_DIV)]);
+
+val DIV_0_IMP_LT = store_thm("DIV_0_IMP_LT",
+  `!b n. 1 < b /\ (n DIV b = 0) ==> n < b`,
+  REPEAT STRIP_TAC \\ SPOSE_NOT_THEN ASSUME_TAC
+    \\ FULL_SIMP_TAC std_ss [NOT_LESS]
+    \\ IMP_RES_TAC LESS_EQUAL_ADD
+    \\ `0 < b` by DECIDE_TAC
+    \\ IMP_RES_TAC ADD_DIV_ADD_DIV
+    \\ POP_ASSUM (SPECL_THEN [`1`,`p`] (ASSUME_TAC o SIMP_RULE std_ss []))
+    \\ FULL_SIMP_TAC arith_ss []);
+
+val lem = prove(
+  `!b n. 1 < b ==> PRE (LENGTH (n2l b n)) <= LENGTH (n2l b (n DIV b))`,
+  SRW_TAC [ARITH_ss] [LENGTH_n2l]
+    << [
+      `0 <= n DIV b /\ 0 < n` by DECIDE_TAC
+        \\ IMP_RES_TAC DIV_0_IMP_LT
+        \\ SRW_TAC [ARITH_ss] [LOG_RWT],
+      IMP_RES_TAC (METIS_PROVE [LESS_DIV_EQ_ZERO,NOT_LESS_EQUAL]
+         ``!b n. 1 < b /\ ~(n DIV b = 0) ==> b <= n``)
+        \\ SRW_TAC [ARITH_ss] [LOG_DIV]]);
+
+val EL_n2l = store_thm("EL_n2l",
+  `!b x n. 1 < b /\ x < LENGTH (n2l b n) ==>
+     (EL x (n2l b n) = (n DIV (b ** x)) MOD b)`,
+  completeInduct_on `LOG b n`
+    \\ SRW_TAC [] []
+    \\ ONCE_REWRITE_TAC [n2l_def]
+    \\ SRW_TAC [ARITH_ss] []
+    << [
+      IMP_RES_TAC LENGTH_n2l
+        \\ Cases_on `n = 0`
+        \\ FULL_SIMP_TAC arith_ss []
+        << [ALL_TAC, `LOG b n = 0` by SRW_TAC [ARITH_ss] [LOG_RWT]]
+        \\ `x = 0` by DECIDE_TAC \\ SRW_TAC [ARITH_ss] [EXP],
+      Cases_on `x = 0`
+        \\ SRW_TAC [ARITH_ss] [EXP, EL_CONS]
+        \\ `LOG b (n DIV b) < LOG b n /\ PRE x < x /\ 0 < x`
+        by SRW_TAC [ARITH_ss] [LOG_DIV_LESS]
+        \\ `PRE x < LENGTH (n2l b (n DIV b))`
+        by METIS_TAC [lem, INV_PRE_LESS, LESS_LESS_EQ_TRANS]
+        \\ RES_TAC
+        \\ POP_ASSUM (SPECL_THEN [`n DIV b`,`b`]
+             (ASSUME_TAC o SIMP_RULE std_ss []))
+        \\ POP_ASSUM (SPEC_THEN `PRE x` IMP_RES_TAC)
+        \\ SRW_TAC [ARITH_ss] [GSYM EXP, DIV_DIV_DIV_MULT,
+             DECIDE ``!n. 0 < n ==> (SUC (PRE n) = n)``]]);
+
+val LIST_EQ = prove(
+  `!a b. (LENGTH a = LENGTH b) /\
+         (!x. x < LENGTH a ==> (EL x a = EL x b)) ==>
+         (a = b)`,
+  Induct_on `a` \\ Induct_on `b` \\ SRW_TAC [] []
+    \\ METIS_TAC [prim_recTheory.LESS_0, LESS_MONO_EQ, EL, HD, TL]);
+
+val n2l_l2n = prove(
+  `!b n l. 1 < b /\ EVERY ($> b) l /\ (n = l2n b l) ==>
+      (n2l b n = if n = 0 then [0] else TAKE (SUC (LOG b n)) l)`,
+  SRW_TAC [] [] >> SRW_TAC [ARITH_ss] [Once n2l_def]
+    \\ MATCH_MP_TAC LIST_EQ \\ IMP_RES_TAC LENGTH_l2n
+    \\ SRW_TAC [ARITH_ss] [LENGTH_n2l,LENGTH_TAKE,EL_TAKE,EL_n2l,l2n_DIGIT]);
+
+val n2l_l2n = save_thm("n2l_l2n",
+  (GEN `b` o GEN `l` o REWRITE_RULE [] o SPECL [`b`,`l2n b l`,`l`]) n2l_l2n);
+
+(* ------------------------------------------------------------------------- *)
+
+val MAP_ID = prove(
+  `!l. EVERY (\x. f x = x) l ==> (MAP f l = l)`,
+  Induct \\ SRW_TAC [] []);
+
+val n2l_BOUND = store_thm("n2l_BOUND",
+  `!b n. 0 < b ==> EVERY ($> b) (n2l b n)`,
+  NTAC 2 STRIP_TAC \\ completeInduct_on `LOG b n`
+    \\ SRW_TAC [ARITH_ss] [Once n2l_def, GREATER_DEF]
+    \\ `LOG b (n DIV b) < LOG b n` by SRW_TAC [ARITH_ss] [LOG_DIV_LESS]
+    \\ SRW_TAC [ARITH_ss] []);
+
+val s2n_n2s = store_thm("s2n_n2s",
+  `!c2n n2c b n. 1 < b /\ (!x. x < b ==> (c2n (n2c x) = x)) ==>
+      (s2n b c2n (n2s b n2c n) = n)`,
+  SRW_TAC [] [s2n_def, n2s_def, MAP_MAP_o]
+    \\ `MAP (c2n o n2c) (n2l b n) = n2l b n`
+    by MATCH_MP_TAC MAP_ID
+    \\ SRW_TAC [ARITH_ss] [l2n_n2l]
+    \\ `!x. ($> b) x ==> (\x. c2n (n2c x) = x) x` by METIS_TAC [GREATER_DEF]
+    \\ IMP_RES_TAC EVERY_MONOTONIC
+    \\ POP_ASSUM MATCH_MP_TAC
+    \\ METIS_TAC [n2l_BOUND, DECIDE ``1 < b ==> 0 < b``]);
+
+(* ......................................................................... *)
+
+val MAP_TAKE = prove(
+  `!f n l. MAP f (TAKE n l) = TAKE n (MAP f l)`,
+  Induct_on `l` \\ SRW_TAC [] []);
+
+val REVERSE_LASTN = prove(
+  `!n l. n <= LENGTH l ==> (LASTN n l = REVERSE (TAKE n (REVERSE l)))`,
+  SRW_TAC [] [FIRSTN_REVERSE]);
+
+val n2s_s2n = store_thm("n2s_s2n",
+  `!c2n n2c b s.
+     1 < b /\ EVERY ($> b o c2n) (EXPLODE s) ==>
+     (n2s b n2c (s2n b c2n s) =
+       if s2n b c2n s = 0 then STRING (n2c 0) ""
+       else TRANSFORM (MAP (n2c o c2n) o LASTN (SUC (LOG b (s2n b c2n s)))) s)`,
+  SRW_TAC [] [s2n_def, n2s_def, TRANSFORM_def]
+    >> SRW_TAC [ARITH_ss] [l2n_def, Once n2l_def]
+    \\ ABBREV_TAC `l = MAP c2n (REVERSE (EXPLODE s))`
+    \\ `~(l = [])` by (STRIP_TAC \\ FULL_SIMP_TAC std_ss [l2n_def])
+    \\ `EVERY ($> b) l` by (UNABBREV_TAC `l`
+          \\ SRW_TAC [] [EVERY_MAP, ALL_EL_REVERSE,
+                         simpLib.SIMP_PROVE std_ss [FUN_EQ_THM]
+                           ``(\x:char. b:num > c2n x) = ($> b o c2n)``])
+    \\ SRW_TAC [] [n2l_l2n]
+    \\ IMP_RES_TAC LENGTH_l2n
+    \\ `SUC (LOG b (l2n b l)) <= LENGTH (EXPLODE s)`
+    by METIS_TAC [LENGTH_MAP, LENGTH_REVERSE]
+    \\ UNABBREV_TAC `l`
+    \\ SRW_TAC [] [GSYM MAP_REVERSE, REVERSE_LASTN, GSYM MAP_TAKE, MAP_MAP_o]);
+
+(* ------------------------------------------------------------------------- *)
+
+val BIT_num_from_bin_list = store_thm("BIT_num_from_bin_list",
+  `!x l. EVERY ($> 2) l /\ x < LENGTH l ==>
+         (BIT x (num_from_bin_list l) = (EL x l = 1))`,
+  SRW_TAC [ARITH_ss]
+    [num_from_bin_list_def, l2n_DIGIT, SUC_SUB, BIT_def, BITS_THM]);
+
+val BIT_num_from_bin_string = store_thm("BIT_num_from_bin_string",
+  `!x s. EVERY ($> 2 o UNHEX) (EXPLODE s) /\ x < STRLEN s ==>
+         (BIT x (num_from_bin_string s) =
+          (UNHEX (s ' (PRE (STRLEN s - x))) = 1))`,
+  SRW_TAC [ARITH_ss] [num_from_bin_string_def, s2n_def]
+    \\ `x < LENGTH (MAP UNHEX (REVERSE (EXPLODE s))) /\
+        x < LENGTH (REVERSE (EXPLODE s)) /\ x < LENGTH (EXPLODE s)`
+    by SRW_TAC [] [LENGTH_MAP, LENGTH_REVERSE, GSYM STRLEN_THM]
+    \\ `EVERY ($> 2) (MAP UNHEX (REVERSE (EXPLODE s)))`
+    by SRW_TAC [] [EVERY_MAP, ALL_EL_REVERSE,
+          simpLib.SIMP_PROVE std_ss [FUN_EQ_THM]
+            ``(\x. 2 > UNHEX x) = ($> 2 o UNHEX)``]
+    \\ SRW_TAC [ARITH_ss]
+         [l2n_DIGIT, EL_MAP, EL_REVERSE, SUC_SUB, BIT_def, BITS_THM, GET,
+          STRLEN_THM]);
+
+val EL_num_to_bin_list = store_thm("EL_num_to_bin_list",
+  `!x n. x < LENGTH (num_to_bin_list n) ==>
+         (EL x (num_to_bin_list n) = BITV n x)`,
+  SRW_TAC [ARITH_ss]
+    [num_to_bin_list_def, EL_n2l, SUC_SUB, BITV_def, BIT_def, BITS_THM]);
+
+val GET_num_to_bin_string = store_thm("GET_num_to_bin_string",
+  `!x n. x < STRLEN (num_to_bin_string n) ==>
+         (num_to_bin_string n ' x =
+          HEX (BITV n (PRE (STRLEN (num_to_bin_string n) - x))))`,
+  SRW_TAC [ARITH_ss]
+       [num_to_bin_string_def, n2s_def, GET, BITV_def, BIT_def, BITS_THM,
+        STRLEN_THM, EXPLODE_IMPLODE, LENGTH_REVERSE, LENGTH_MAP, SUC_SUB]
+    \\ `PRE (LENGTH (n2l 2 n) - x) < LENGTH (n2l 2 n)`
+    by (SIMP_TAC arith_ss [PRE_SUB1] \\ SIMP_TAC arith_ss [LENGTH_n2l])
+    \\ SRW_TAC [ARITH_ss] [EL_REVERSE, EL_MAP, EL_n2l, SUC_SUB]);
+
+(* ------------------------------------------------------------------------- *)
+
+val LESS_THM =
+  CONV_RULE numLib.SUC_TO_NUMERAL_DEFN_CONV prim_recTheory.LESS_THM;
+
+val UNHEX_HEX = store_thm("UNHEX_HEX",
+  `!n. n < 16 ==> (UNHEX (HEX n) = n)`, SRW_TAC [] [LESS_THM] \\ EVAL_TAC);
+
+val HEX_UNHEX = store_thm("HEX_UNHEX",
+  `!c. isHexDigit c ==> (HEX (UNHEX c) = toUpper c)`,
+  Cases \\ SRW_TAC [] [isHexDigit_def] \\ PAT_ASSUM `n < 256` (K ALL_TAC)
+    << [`n < 58` by DECIDE_TAC, `n < 103` by DECIDE_TAC,
+        `n < 71` by DECIDE_TAC]
+    \\ FULL_SIMP_TAC std_ss [LESS_THM]
+    \\ FULL_SIMP_TAC arith_ss []
+    \\ EVAL_TAC);
+
+val DEC_UNDEC = store_thm("DEC_UNDEC",
+  `!c. isDigit c ==> (HEX (UNHEX c) = c)`,
+  Cases \\ SRW_TAC [] [isDigit_def] \\ PAT_ASSUM `n < 256` (K ALL_TAC)
+    \\ `n < 58` by DECIDE_TAC
+    \\ FULL_SIMP_TAC std_ss [LESS_THM]
+    \\ FULL_SIMP_TAC arith_ss []
+    \\ EVAL_TAC);
+
+val rwts = [FUN_EQ_THM, UNHEX_HEX, l2n_n2l, s2n_n2s,
+  num_from_bin_list_def,num_from_oct_list_def,num_from_dec_list_def,
+  num_from_hex_list_def,num_to_bin_list_def,num_to_oct_list_def,
+  num_to_dec_list_def,num_to_hex_list_def,num_from_bin_string_def,
+  num_from_oct_string_def,num_from_dec_string_def,num_from_hex_string_def,
+  num_to_bin_string_def,num_to_oct_string_def,num_to_dec_string_def,
+  num_to_hex_string_def];
+
+val num_bin_list = store_thm("num_bin_list",
+  `num_from_bin_list o num_to_bin_list = I`, SRW_TAC [ARITH_ss] rwts);
+val num_oct_list = store_thm("num_oct_list",
+  `num_from_oct_list o num_to_oct_list = I`, SRW_TAC [ARITH_ss] rwts);
+val num_dec_list = store_thm("num_dec_list",
+  `num_from_dec_list o num_to_dec_list = I`, SRW_TAC [ARITH_ss] rwts);
+val num_hex_list = store_thm("num_hex_list",
+  `num_from_hex_list o num_to_hex_list = I`, SRW_TAC [ARITH_ss] rwts);
+
+val num_bin_string = store_thm("num_bin_string",
+  `num_from_bin_string o num_to_bin_string = I`, SRW_TAC [ARITH_ss] rwts);
+val num_oct_string = store_thm("num_oct_string",
+  `num_from_oct_string o num_to_oct_string = I`, SRW_TAC [ARITH_ss] rwts);
+val num_dec_string = store_thm("num_dec_string",
+  `num_from_dec_string o num_to_dec_string = I`, SRW_TAC [ARITH_ss] rwts);
+val num_hex_string = store_thm("num_hex_string",
+  `num_from_hex_string o num_to_hex_string = I`, SRW_TAC [ARITH_ss] rwts);
 
 (* ------------------------------------------------------------------------- *)
 
